IsaSAT: avoid interference of init rules

Weidenbach_Book/Array_Array_List64.thy
@@ -513,12 +513,14 @@ sepref_definition
   supply [[goals_limit = 1]]
   by sepref
 
+definition init_lrl64 :: \<open>nat \<Rightarrow> _\<close> where
+[simp]: \<open>init_lrl64 = init_lrl\<close>
 
-lemma arrayO_ara_empty_sz_init_lrl: \<open>arrayO_ara_empty_sz n = init_lrl n\<close>
+lemma arrayO_ara_empty_sz_init_lrl: \<open>arrayO_ara_empty_sz n = init_lrl64 n\<close>
   by (induction n) (auto simp: arrayO_ara_empty_sz_def init_lrl_def)
 
 lemma arrayO_raa_empty_sz_init_lrl[sepref_fr_rules]:
-  \<open>(arrayO_ara_empty_sz_code, RETURN o init_lrl) \<in>
+  \<open>(arrayO_ara_empty_sz_code, RETURN o init_lrl64) \<in>
     nat_assn\<^sup>k \<rightarrow>\<^sub>a arrayO_assn (arl64_assn R)\<close>
   using arrayO_ara_empty_sz_code.refine unfolding arrayO_ara_empty_sz_init_lrl .
 
